Verify some generics examples that now translate (#244)
Adds translations from goose-lang/goose#93 and verifies some simple specs for the new generics unit tests. This helped find a few bugs in missing support and incorrect arguments, which are hard to spot by inspection.

There are some oddities in these proofs (e.g. unexpectedly shelved instances) that aren't great but they don't seem specifically related to generics and we can debug them separately.

new/code/github_com/goose_lang/goose/testdata/examples/unittest/generics.v
@@ -13,6 +13,52 @@ Definition Box : val :=
     (#"Value"%go, "T")
   ].
 
+(* BoxGet is a function getter (rather than a method)
+
+   go: generics.go:9:6 *)
+Definition BoxGet : val :=
+  rec: "BoxGet" "T" "b" :=
+    exception_do (let: "b" := (mem.alloc "b") in
+    return: (!["T"] (struct.field_ref (Box "T") #"Value"%go "b"))).
+
+(* go: generics.go:13:6 *)
+Definition BoxGet2 : val :=
+  rec: "BoxGet2" "b" :=
+    exception_do (let: "b" := (mem.alloc "b") in
+    return: (![#uint64T] (struct.field_ref (Box #uint64T) #"Value"%go "b"))).
+
+(* go: generics.go:17:17 *)
+Definition Box__Get : val :=
+  rec: "Box__Get" "b" "T" <> :=
+    exception_do (let: "b" := (mem.alloc "b") in
+    return: (!["T"] (struct.field_ref (Box "T") #"Value"%go "b"))).
+
+(* go: generics.go:21:6 *)
+Definition makeGenericBox : val :=
+  rec: "makeGenericBox" "T" "value" :=
+    exception_do (let: "value" := (mem.alloc "value") in
+    return: (let: "$Value" := (!["T"] "value") in
+     struct.make (Box "T") [{
+       "Value" ::= "$Value"
+     }])).
+
+(* go: generics.go:25:6 *)
+Definition makeBox : val :=
+  rec: "makeBox" <> :=
+    exception_do (return: (let: "$Value" := #(W64 42) in
+     struct.make (Box #uint64T) [{
+       "Value" ::= "$Value"
+     }])).
+
+(* go: generics.go:30:6 *)
+Definition useBoxGet : val :=
+  rec: "useBoxGet" <> :=
+    exception_do (let: "x" := (mem.alloc (type.zero_val (Box #uint64T))) in
+    let: "$r0" := (let: "$a0" := #(W64 42) in
+    ((func_call #generics.generics #"makeGenericBox"%go) #uint64T) "$a0") in
+    do:  ("x" <-[Box #uint64T] "$r0");;;
+    return: ((method_call #generics.generics #"Box" #"Get" (![Box #uint64T] "x") #uint64T) #())).
+
 Definition Container : val :=
   λ: "T", type.structT [
     (#"X"%go, "T");
@@ -20,6 +66,32 @@ Definition Container : val :=
     (#"Z"%go, #ptrT);
     (#"W"%go, #uint64T)
   ].
+
+(* go: generics.go:43:6 *)
+Definition useContainer : val :=
+  rec: "useContainer" <> :=
+    exception_do (let: "container" := (mem.alloc (type.zero_val (Container #uint64T))) in
+    let: "$r0" := (let: "$X" := #(W64 1) in
+    let: "$Y" := ((let: "$v0" := #(W64 2) in
+    let: "$k0" := #(W64 1) in
+    map.literal #intT #uint64T [("$k0", "$v0")])) in
+    let: "$Z" := (mem.alloc (type.zero_val #uint64T)) in
+    let: "$W" := #(W64 3) in
+    struct.make (Container #uint64T) [{
+      "X" ::= "$X";
+      "Y" ::= "$Y";
+      "Z" ::= "$Z";
+      "W" ::= "$W"
+    }]) in
+    do:  ("container" <-[Container #uint64T] "$r0");;;
+    let: "$r0" := #(W64 2) in
+    do:  ((struct.field_ref (Container #uint64T) #"X"%go "container") <-[#uint64T] "$r0");;;
+    let: "$r0" := #(W64 3) in
+    do:  (map.insert (![type.mapT #intT #uint64T] (struct.field_ref (Container #uint64T) #"Y"%go "container")) #(W64 2) "$r0");;;
+    let: "$r0" := (mem.alloc (type.zero_val #uint64T)) in
+    do:  ((struct.field_ref (Container #uint64T) #"Z"%go "container") <-[#ptrT] "$r0");;;
+    let: "$r0" := #(W64 4) in
+    do:  ((struct.field_ref (Container #uint64T) #"W"%go "container") <-[#uint64T] "$r0")).
 
 Definition UseContainer : val :=
   λ: <>, type.structT [
@@ -32,11 +104,61 @@ Definition OnlyIndirect : val :=
     (#"Y"%go, #ptrT)
   ].
 
+Definition MultiParam : val :=
+  λ: "A" "B", type.structT [
+    (#"Y"%go, "B");
+    (#"X"%go, "A")
+  ].
+
+(* go: generics.go:71:6 *)
+Definition useMultiParam : val :=
+  rec: "useMultiParam" <> :=
+    exception_do (let: "mp" := (mem.alloc (type.zero_val (MultiParam #uint64T #boolT))) in
+    let: "$r0" := (let: "$Y" := #true in
+    let: "$X" := #(W64 1) in
+    struct.make (MultiParam #uint64T #boolT) [{
+      "Y" ::= "$Y";
+      "X" ::= "$X"
+    }]) in
+    do:  ("mp" <-[MultiParam #uint64T #boolT] "$r0");;;
+    let: "$r0" := #(W64 2) in
+    do:  ((struct.field_ref (MultiParam #uint64T #boolT) #"X"%go "mp") <-[#uint64T] "$r0")).
+
+(* go: generics.go:76:6 *)
+Definition swapMultiParam : val :=
+  rec: "swapMultiParam" "A" "p" :=
+    exception_do (let: "p" := (mem.alloc "p") in
+    let: "temp" := (mem.alloc (type.zero_val "A")) in
+    let: "$r0" := (!["A"] (struct.field_ref (MultiParam "A" "A") #"X"%go (![#ptrT] "p"))) in
+    do:  ("temp" <-["A"] "$r0");;;
+    let: "$r0" := (!["A"] (struct.field_ref (MultiParam "A" "A") #"Y"%go (![#ptrT] "p"))) in
+    do:  ((struct.field_ref (MultiParam "A" "A") #"X"%go (![#ptrT] "p")) <-["A"] "$r0");;;
+    let: "$r0" := (!["A"] "temp") in
+    do:  ((struct.field_ref (MultiParam "A" "A") #"Y"%go (![#ptrT] "p")) <-["A"] "$r0")).
+
+(* go: generics.go:82:6 *)
+Definition multiParamFunc : val :=
+  rec: "multiParamFunc" "A" "B" "x" "b" :=
+    exception_do (let: "b" := (mem.alloc "b") in
+    let: "x" := (mem.alloc "x") in
+    return: ((let: "$sl0" := (!["B"] "b") in
+     slice.literal "B" ["$sl0"]))).
+
+(* go: generics.go:86:6 *)
+Definition useMultiParamFunc : val :=
+  rec: "useMultiParamFunc" <> :=
+    exception_do (do:  (let: "$a0" := #(W64 1) in
+    let: "$a1" := #true in
+    ((func_call #generics.generics #"multiParamFunc"%go) #uint64T #boolT) "$a0" "$a1");;;
+    return: (#())).
+
 Definition vars' : list (go_string * go_type) := [].
 
-Definition functions' : list (go_string * val) := [].
+Definition functions' : list (go_string * val) := [("BoxGet"%go, BoxGet); ("BoxGet2"%go, BoxGet2); ("makeGenericBox"%go, makeGenericBox); ("makeBox"%go, makeBox); ("useBoxGet"%go, useBoxGet); ("useContainer"%go, useContainer); ("useMultiParam"%go, useMultiParam); ("swapMultiParam"%go, swapMultiParam); ("multiParamFunc"%go, multiParamFunc); ("useMultiParamFunc"%go, useMultiParamFunc)].
 
-Definition msets' : list (go_string * (list (go_string * val))) := [("Box"%go, []); ("Box'ptr"%go, []); ("Container"%go, []); ("Container'ptr"%go, []); ("UseContainer"%go, []); ("UseContainer'ptr"%go, []); ("OnlyIndirect"%go, []); ("OnlyIndirect'ptr"%go, [])].
+Definition msets' : list (go_string * (list (go_string * val))) := [("Box"%go, [("Get"%go, Box__Get)]); ("Box'ptr"%go, [("Get"%go, (λ: "$recvAddr",
+                 method_call #generics.generics #"Box" #"Get" (![Box #()] "$recvAddr")
+                 )%V)]); ("Container"%go, []); ("Container'ptr"%go, []); ("UseContainer"%go, []); ("UseContainer'ptr"%go, []); ("OnlyIndirect"%go, []); ("OnlyIndirect'ptr"%go, []); ("MultiParam"%go, []); ("MultiParam'ptr"%go, [])].
 
 #[global] Instance info' : PkgInfo generics.generics :=
   {|
