new/should_build.v
@@ -1,10 +1,11 @@
-From New.code.go_etcd_io.raft Require v3.
 From New.generatedproof.github_com.goose_lang.goose.testdata.examples
-  Require unittest unittest.generics semantics.
+  Require unittest semantics.
 (* required just to make sure this demo works *)
 From New.golang.theory Require static_mem.
 From New.proof Require go_etcd_io.etcd.raft.v3.
 From New.proof.github_com.mit_pdos.gokv Require partialapp asyncfile lockservice globals_test.
+From New.proof.github_com.goose_lang.goose.testdata.examples
+  Require unittest.generics.
 
 From New.proof Require go_etcd_io.etcd.client.v3.leasing.
 From New.proof Require Import chan context.
